@prefix : <http://www.monnet-project.eu/lemon-morphology#> .
@prefix rdfs: <http://www.w3.org/2000/01/rdf-schema#> .
@prefix lemon-morphology: <http://www.monnet-project.eu/lemon-morphology#> .
@prefix owl2xml: <http://www.w3.org/2006/12/owl2-xml#> .
@prefix owl: <http://www.w3.org/2002/07/owl#> .
@prefix xsd: <http://www.w3.org/2001/XMLSchema#> .
@prefix rdf: <http://www.w3.org/1999/02/22-rdf-syntax-ns#> .
@prefix lemon: <http://www.monnet-project.eu/lemon#> .
@base <http://www.monnet-project.eu/lemon-morphology> .

<http://www.monnet-project.eu/lemon-morphology> rdf:type owl:Ontology ;
                                                
                                                owl:imports <http://www.monnet-project.eu/lemon> .


#################################################################
#
#    Object Properties
#
#################################################################


###  http://www.monnet-project.eu/lemon#property

lemon:property rdf:type owl:ObjectProperty .



###  http://www.monnet-project.eu/lemon-morphology#generates

:generates rdf:type owl:ObjectProperty ;
           
           rdfs:comment "Indicates the prototype for the output form generated by the morphological transform"@en ;
           
           rdfs:domain :MorphTransform ;
           
           rdfs:range :Prototype .



###  http://www.monnet-project.eu/lemon-morphology#nextScope

:nextScope rdf:type owl:ObjectProperty ;
           
           rdfs:comment "Indicates a transform that may be applied on the result of the transform. This is known as polysynthesis."@en ;
           
           rdfs:domain :MorphTransform ;
           
           rdfs:range :MorphTransform .



###  http://www.monnet-project.eu/lemon-morphology#onStem

:onStem rdf:type owl:ObjectProperty ;
        
        rdfs:comment "Indicates the prototype for the input form used by this transform"@en ;
        
        rdfs:domain :MorphTransform ;
        
        rdfs:range :Prototype .



###  http://www.monnet-project.eu/lemon-morphology#pattern

:pattern rdf:type owl:ObjectProperty ;
         
         rdfs:comment "Indicate the set of morphological transforms a lexical entry may go under"@en ;
         
         rdfs:domain lemon:LexicalEntry ;
         
         rdfs:range :MorphPattern .



###  http://www.monnet-project.eu/lemon-morphology#transform

:transform rdf:type owl:ObjectProperty ;
           
           rdfs:comment "Indicates a single transform in a morphological pattern"@en ;
           
           rdfs:domain :MorphPattern ;
           
           rdfs:range :MorphTransform .





#################################################################
#
#    Data properties
#
#################################################################


###  http://www.monnet-project.eu/lemon-morphology#rule

:rule rdf:type owl:DatatypeProperty ;
      
      rdfs:comment "A regular expression that describes the transform the format for this is _~_/_~_ where the left hand side of the slash indicates the matcher and the right the replacement. The tilde indicates the original stem and _ may be any valid regular expression. For agglutantive morphology + is used to indicate the boundry between the pattern's lexical entry and the lexical entry to fuse with"@en ;
      
      rdfs:domain :MorphTransform ;
      
      rdfs:range xsd:string .





#################################################################
#
#    Classes
#
#################################################################


###  http://www.monnet-project.eu/lemon#LemonElement

lemon:LemonElement rdf:type owl:Class .



###  http://www.monnet-project.eu/lemon#LexicalEntry

lemon:LexicalEntry rdf:type owl:Class .



###  http://www.monnet-project.eu/lemon-morphology#MorphPattern

:MorphPattern rdf:type owl:Class ;
              
              rdfs:subClassOf lemon:LemonElement ,
                              [ rdf:type owl:Restriction ;
                                owl:onProperty :transform ;
                                owl:minCardinality "1"^^xsd:nonNegativeInteger
                              ] ;
              
              rdfs:comment "Morphological patterns consist of sets of transform that can be applied to the forms of a lexical entry to generate new forms."@en .



###  http://www.monnet-project.eu/lemon-morphology#MorphTransform

:MorphTransform rdf:type owl:Class ;
                
                rdfs:subClassOf lemon:LemonElement ,
                                [ rdf:type owl:Restriction ;
                                  owl:onProperty :rule ;
                                  owl:minCardinality "1"^^xsd:nonNegativeInteger
                                ] ;
                
                rdfs:comment "Transforms apply to a form of a lexical entry to create a new form"@en .



###  http://www.monnet-project.eu/lemon-morphology#Prototype

:Prototype rdf:type owl:Class ;
           
           rdfs:subClassOf lemon:LemonElement ,
                           [ rdf:type owl:Restriction ;
                             owl:onProperty lemon:property ;
                             owl:minCardinality "1"^^xsd:nonNegativeInteger
                           ] ;
           
           rdfs:comment "Prototypes are abstract forms without representation used in morphology to describe the input and output transforms of the morphological transform"@en .



###  http://www.w3.org/2002/07/owl#Thing

owl:Thing rdf:type owl:Class .




###  Generated by the OWL API (version 2.2.1.1138) http://owlapi.sourceforge.net

